\documentclass[letter]{article}
\usepackage[monocolor]{ahsansabit}

\title{Computational Complex Analysis : : Class 29}
\author{Ahmed Saad Sabit, Rice University}
\date{\today}

\begin{document}
\maketitle
Last class we found that, 
\[
\frac{1}{\Gamma(z)} = \lim_{n \to \infty} {z(z+1) \cdots (z+n) \over n^{z} n!}
\]
Valid for all $z \in \mathbb{C}$. People use the word entire holomorphic function. Slang for holomorphic function defined on the ``entire" complex plane. We can rewrite this as an infinite product, 
\[
\prod_{n=1}^{\infty}   \phi_n = \lim_{W \to \infty} \prod_{n=1}^{N}  \phi_n 
\]
\[
	{ z ( z+1) \cdots (z+n) \over n^{z} n!} = \frac{z}{n^z} { \frac{z+1}{1} \frac{z+2}{2} \cdots \frac{z+n}{n}}
\] The above thing diverges. Weierstrass does this, 
\[
 = z {
	 \left(1 + \frac{z}{1}\right)e^{- \frac{z}{1}} 
	 \left(1 + \frac{z}{2}\right)e^{- \frac{z}{2}}
	 \cdots 
	 \left(1 + \frac{z}{n}\right)e^{- \frac{z}{n}}
	 \over 
	 n^{z}
 } 
 e^{z \left(1 + \frac{1}{2} + \cdots + \frac{1}{n}\right)}
\]
The upper right thing blows up.  
\[
 = z {
	 \left(1 + \frac{z}{1}\right)e^{- \frac{z}{1}} 
	 \left(1 + \frac{z}{2}\right)e^{- \frac{z}{2}}
	 \cdots 
	 \left(1 + \frac{z}{n}\right)e^{- \frac{z}{n}}
	 \over 
	 e^{ z \ln n}
 } 
 e^{z \left(1 + \frac{1}{2} + \cdots + \frac{1}{n}\right)}
\]
\[
 = z \left({
	 \left(1 + \frac{z}{1}\right)e^{- \frac{z}{1}} 
	 \left(1 + \frac{z}{2}\right)e^{- \frac{z}{2}}
	 \cdots 
	 \left(1 + \frac{z}{n}\right)e^{- \frac{z}{n}}
 }\right) 
 e^{z \left(1 + \frac{1}{2} + \cdots + \frac{1}{n}\right)} 
 e^{-z \ln n}
\]
So what we can write now is that, 
\[
\frac{z(z+1)(\cdots)(z+n)}{n^{z}n!} = 
z \prod_{k= 1}^{n} \left(1 + \frac{z}{k}\right)e^{-z / k } 
\times 
\left(
e^{z (1 + 1 / 2 + \cdots + 1 / n) - \ln n} 
\right)
\]  

The thing goes to limit, 
\[
1 + 1 / 2 + \cdots + 1 / n - \ln(n) \to \gamma
\]
$\gamma$ is the  \textbf{Euler-Mascheroni} Number.

There is a limit hence, 
\[
\boxed{
\frac{1}{\Gamma (z)} = 
z e^{ \gamma z} \prod_{k=1}^{\infty} \left(1 + \frac{z}{k}\right)e^{- \frac{z}{k}} }
\]
We had in last class, 
\[
\Gamma(a) \Gamma(1-a) = \frac{\pi}{\sin \pi a} \qquad \left(0 < a < 1\right)
\]
\[
\frac{\pi}{\sin \pi z}
	= \Gamma(z) \Gamma(1-z) = 
\lim \frac{n^{z} n!}{z(z+1)\cdots (z+n)} 
\lim \frac{n^{1-z} n!}{(1-z)(2-z)\cdots (n+1-z)} 
\]
\[
= \lim 
\frac{n (n!)^2 \quad (-1)^{n}}{z (z+1)(\cdots)(z+n) \times (z-1)(z-2)(\cdots)(z-n-1)}
\]
\[
= \lim
\frac{n(n!)^2 \quad (-1)^{n+1}}{z (z^2 - 1) (z^2 - 4) (\cdots) (z^2-n^2)} \frac{1}{z -n - 1}
\]
\[=
\lim 
\frac{n (n!)^2 \quad (-1)}{z (1-z^2) (\cdots)(n^2-z^2)} \frac{1}{z-n-1}
\]
\[
= \lim 
\frac{1}{z 
\left(1 - \frac{z^2}{1}\right)\left(1 - \frac{z^2}{2^2}\right) \left(\cdots\right) \left(1 - \frac{z^2}{n^2}\right)} \frac{1}{z - n -1 }
\]
\[
\frac{\sin \pi z}{\pi z } = \prod_{n=1}^{\infty} 
\left(1- \frac{z^2}{n^2}\right)
\] 


\end{document}
