\documentclass[letter, 10pts]{article}
\usepackage[monocolor]{../math232/ahsansabit}
\usepackage[]{float}
\usepackage{tikz}
\usepackage{tikz-3dplot}
\usepackage[outline]{contour} % glow around text
\usepackage{xcolor}
\usepackage{pdfpages}
\usepackage{physics}
\usepackage[]{array}
\newcolumntype{C}{>{\centering\arraybackslash}m{2cm}}
\renewcommand{\arraystretch}{2.5} 
\usepackage{multicol}
\title{Quantum Mechanics : : Homework 0X}
\author{Ahmed Saad Sabit, Rice University}
\date{\today}
\newcommand{\hb}{\hbar}
\newcommand{\U}{\uparrow}
\newcommand{\D}{\downarrow}
\usepackage[]{braket}
\begin{document}
\maketitle

























\section*{Problem 01} 
\hrule
\subsection*{(a)} 
I always feel weird to use $\hat{P}$ operator
\begin{align*}
	\braket{\vec{r} | \hat{P_x} | E, m} &= - i \hb \frac{\mathrm{d} \Psi_{E,m}(r)}{\mathrm{d} x} \\
	\braket{\vec{r} | \hat{X}^2 | E, m} &= \braket{\vec{r} | \hat{X}^2 | \vec{r}} \braket{\vec{r} | E,m}  \\
					    &= x^2 \Psi_{E,m} (r) \\
\end{align*}
Hence 
\begin{align*}
	\braket{\vec{r} | \hat{H} | E,m} = E \Psi_{E,m}(r) &= 
\frac{- \hb^2}{2 \mu}
\left(
	\nabla^2 \Psi_{E,m}(r) \right) 
	+ \frac{\mu \omega^2}{2} \left(x^2 + y^2\right) \Psi_{E,m}(r)
\\
				 &= 
				 \frac{- \hb^2}{2 \mu}
\left(
	\frac{\mathrm{d} ^2}{\mathrm{d} r^2} 
	- 
	\frac{m^2}{r^2}
	+ 
	\frac{1}{r} \frac{\mathrm{d} }{\mathrm{d} r}
\right) \Psi_{E,m} (r)
	+ \frac{\mu \omega^2}{2} r^2 \Psi_{E,m}(r)
\\
				 &= 
				 \frac{- \hb^2}{2 \mu}
\left(
	\frac{\mathrm{d} ^2}{\mathrm{d} r^2} 
	- 
	\frac{m^2}{r^2}
	+ 
	\frac{1}{r} \frac{\mathrm{d} }{\mathrm{d} r}
	- \frac{2 \mu}{\hb} \frac{\mu \omega^2}{2} r^2 \right) \Psi_{E,m}(r)
\\
				 &\implies 
				\frac{- \hb^2}{2 \mu}
\left(
	\frac{\mathrm{d} ^2}{\mathrm{d} r^2} 
	- 
	\frac{m^2}{r^2}
	+ 
	\frac{1}{r} \frac{\mathrm{d} }{\mathrm{d} r}
	-  \frac{\mu ^2 \omega^2}{\hb} r^2 + \frac{2\mu}{\hb^2} E \right) \Psi_{E,m}(r) 
	= 0
\\
				 &= -\omega \hb b^2
\left(
	\frac{\mathrm{d} ^2}{\mathrm{d} r^2} 
	- 
	\frac{m^2}{r^2}
	+ 
	\frac{1}{r} \frac{\mathrm{d} }{\mathrm{d} r}
	-  \frac{\mu ^2 \omega^2}{\hb} r^2 + \frac{2\mu}{\hb^2} E \right) \Psi_{E,m}(r) 
	= 0
\\
				 &= 
\left(
	\frac{\mathrm{d} ^2}{\mathrm{d} y^2} 
	- 
	\frac{m^2}{y^2}
	+ 
	\frac{1}{y} \frac{\mathrm{d} }{\mathrm{d} y}
	-   y^2 + \frac{2\mu}{\hb^2} \frac{\hb}{\mu \omega} E \right) \Psi_{E,m}(r) 
	= 0
\\
				 &=
\left(
	\frac{\mathrm{d} ^2}{\mathrm{d} y^2} 
	- 
	\frac{m^2}{y^2}
	+ 
	\frac{1}{y} \frac{\mathrm{d} }{\mathrm{d} y}
	-   y^2 + \frac{2}{\hb \omega} E \right) \Psi_{E,m}(r) 
	= 0
\\
\end{align*}
\[
\boxed{
\left[
\frac{\mathrm{d} ^2}{\mathrm{d} y^2}
+ 
\frac{1}{y} \frac{\mathrm{d} }{\mathrm{d} y}
- 
\frac{m^2}{y^2}
- y^2 + 
2 \varepsilon 
\right]
\psi_{\varepsilon, m}(y) = 0
}
\] 








\subsection*{(b)} 
\[
\left[
\frac{\mathrm{d} ^2}{\mathrm{d} y^2}
+ 
\frac{1}{y} \frac{\mathrm{d} }{\mathrm{d} y}
- 
\frac{m^2}{y^2}
+ 
2 \varepsilon 
\right]
y^{\alpha}
= 0
\] 
\begin{align*}
\alpha (\alpha - 1) y^{\alpha - 2} + 
\alpha y^{\alpha - 2} - 
m^2 y^{\alpha - 2} + 
2 \varepsilon y^{\alpha} &= 0 
\\
\alpha (\alpha - 1) + 
\alpha  - 
m^2  + 
2 \varepsilon y^{\alpha - \alpha + 2} &= 0 
\\
\alpha^2 
- 
m^2  + 
2 \varepsilon y^{2} &= 0 
\implies
\lim_{y \to 0} \alpha^2 - m^2 + 2 \varepsilon y^2 = 0
\\
		    &\implies \alpha = |m|
\end{align*}
\[
\boxed{
	\lim_{y \to 0} \psi_{\varepsilon, m}(y) = y^{|m|}
}
\] 






\subsection*{(c)}
\begin{align*}
\left[
\frac{\mathrm{d} ^2}{\mathrm{d} y^2}
+ 
\frac{1}{y} \frac{\mathrm{d} }{\mathrm{d} y}
- 
\frac{m^2}{y^2}
+ 
2 \varepsilon 
\right]
y^{|m|}f(y)
&= 0 
\\
\frac{\mathrm{d} }{\mathrm{d} y}
\left(
|m|y^{|m| - 1} f(y) + y^{|m|} f'(y)
\right)
+ \frac{1}{y} \left(
|m|y^{|m| - 1} f(y) + y^{|m|} f'(y)
\right)
- \frac{m^2}{y^2} y^{|m|}f(y) 
	+ 2 \varepsilon y^{|m|}f(y) &= 0
\\
\frac{\mathrm{d} }{\mathrm{d} y}
\left(
|m|y^{|m| - 1} f(y) + y^{|m|} f'(y)
\right)
+ \left(
|m|y^{|m| - 2} f(y) + y^{|m|-1} f'(y)
\right)
- m^2 y^{|m| - 2 }f(y) 
	+ 2 \varepsilon y^{|m|}f(y) &= 0
\\
\left(
|m|(|m| - 1 ) y^{|m| - 2} f(y) 
+ |m| y^{|m| - 1} f'(y) + 
|m| y^{|m| - 1} f'(y)
+ 
y^{|m|}f''(y) 
\right) + \\ 
+ \left(
|m|y^{|m| - 2} f(y) + y^{|m|-1} f'(y)
\right)
- m^2 y^{|m| - 2 }f(y) 
	+ 2 \varepsilon y^{|m|}f(y) &= 0
	\\
y^{|m| - 2} f(y)
\Big[
|m| (|m| - 1)  +
|m|  
- 
m^2  
\Big]
+
y^{|m| - 1}  f'(y)
\Big[
2 |m| + 1 
\Big]
+ 
y^{|m|} 
\Big[
f''(y) + 2 \varepsilon f(y)
\Big] &= 0 \\
y^{|m| - 1}  f'(y)
\Big[
2 |m| + 1 
\Big]
+ 
y^{|m|} 
\Big[
f''(y) + 2 \varepsilon f(y)
\Big] &= 0 \\
f'(y)
\Big[
2 |m| + 1 
\Big]
+ 
y
\Big[
f''(y) + 2 \varepsilon f(y)
\Big] &= 0 \\
f'(y)
\frac{\Big[
2 |m| + 1 
\Big]}{y}
+ 
\Big[
f''(y) + 2 \varepsilon f(y)
\Big] &= 0 \\
\frac{\mathrm{d} }{\mathrm{d} y} 
\left(
e^{- y^2 / 2} u(y) 
\right)
\frac{\Big[
2 |m| + 1 
\Big]}{y}
+ 
\Big[
\frac{\mathrm{d} ^2}{\mathrm{d} y^2} 
\left(
e^{ - y^2 / 2 } u(y) 
\right)+ 2 \varepsilon 
\left(e^{ - y^2 / 2} u(y) \right)
\Big] &= 0 \\
\left(
- y  u(y) +  u'(y) 
\right)e^{ - y^2 / 2}
\frac{\Big[
2 |m| + 1 
\Big]}{y}+  \\ 
+ 
\Big[
\left(
	-u(y) - y u'(y) + u''(y) + y^2 u(y) - y u'(y)  
\right)e^{ - y^2 / 2 } 
+ 2 \varepsilon 
\left(e^{ - y^2 / 2} u(y) \right)
\Big] &= 0 \\
\
\
\
\left(
- y  u(y) +  u'(y) 
\right) 
\frac{\Big[
2 |m| + 1 
\Big]}{y}+  \\ 
+ 
\Big[
\left(
	-u(y) - 2 y u'(y) + u''(y) + y^2 u(y) 
\right) 
+ 2 \varepsilon 
u(y) 
\Big] &= 0 \\
\
\
\
u''(y)+
\left[
\frac{2|m| + 1}{y} - 2y 	
\right] u'
+ 
(2 \varepsilon - 1 - 2|m| - 1) u = 0\\ 
\end{align*}

\[
\boxed{
u''(y)+
\left[
\frac{2|m| + 1}{y} - 2y 	
\right] u'
+ 
(2 \varepsilon - 2|m| - 2) u = 0\\ 
}
\] 


\subsection*{(c)} 
\begin{align*}
u(y) &= \sum_{p = 0}^{\infty} c_p y^{p} \\
u'(y) &= \sum_{p = 1}^{\infty}  p c_p y^{ p - 1}
      = \sum_{p = 0 }^{\infty} (p+1) c_{p+1} y^{p} \\
u''(y) &= \sum_{p = 2}^{\infty}  p(p-1) c_p y^{ p - 2}  
= \sum_{p = 0}^{\infty}  (p+2)(p+1) c_{p+2} y^{ p}  \\ &
\end{align*}
\[
u''(y)+
\left[
\frac{2|m| + 1}{y} - 2y 	
\right] u'
+ 
(2 \varepsilon - 2|m| - 2) u = 0 \] 
\begin{align*}
0 &= 
\sum_{p = 0}^{\infty}  (p+2)(p+1) c_{p+2} y^{ p}  +
\left[
\frac{2|m| + 1}{y} - 2y 	
\right] 
      \sum_{p = 0 }^{\infty} (p+1) c_{p+1} y^{p} 
      + 
(2 \varepsilon - 2|m| - 2) 
\sum_{p = 0}^{\infty} c_p y^{p} 
\\
&= 
\sum_{p = 0}^{\infty}  (p+2)(p+1) c_{p+2} y^{ p}  +
\underbrace{\left[
	({2|m| + 1})
      \sum_{p = -1 }^{\infty} (p+2) c_{p+2} y^{p} 
	- 2  	
      \sum_{p = 0 }^{\infty} (p) c_{p} y^{p} 
\right]}_{\text{term of interest where $c_1 = 0$}}
      + 
(2 \varepsilon - 2|m| - 2) 
\sum_{p = 0}^{\infty} c_p y^{p} 
\\
&= 
\sum_{p = 0}^{\infty}  (p+2)(p+1) c_{p+2} y^{ p}  +
	({2|m| + 1})
      \sum_{p = 0 }^{\infty} (p+2) c_{p+2} y^{p} 
	- 2  	
      \sum_{p = 0 }^{\infty} (p) c_{p} y^{p} 
      + 
(2 \varepsilon - 2|m| - 2) 
\sum_{p = 0}^{\infty} c_p y^{p} 
\\ &=
\sum_{p = 0}^{\infty} y^{p} 
\Biggr[
(p+2)(p+1) c_{p+2} + (2|m|+1) (p+2)c_{p+2} - 2 p c_p + (2 \varepsilon - 2 |m| - 2) c_p
\Biggr]
\\ &=
\sum_{p = 0}^{\infty} y^{p} 
\Biggr[
\underbrace{\left[(p+2)(p+1)  + (2|m|+1) (p+2)\right] 
}_{\text{two terms above}}c_{p+2}
+
\left[ 
- 2 p  + (2 \varepsilon - 2 |m| - 2) \right]
c_p
\Biggr]
\end{align*}
Requirement to keep everything $0$ (also note $p = 2k$) 
\begin{align*}
	c_{p+2}
	&= 
	\frac{
 2 p  - (2 \varepsilon - 2 |m| - 2) 
	}
	{(p+2)(p+1)  + (2|m|+1) (p+2)} \\ 
&=  \frac{
	2p - (2 \varepsilon - 2 |m| - 2)  
}{p^2 + p + 2p + 2 + 2 |m| p + 4 |m|+ p + 2}
	\\
&=  \frac{
	2p - (2 \varepsilon - 2 |m| - 2)  
}{p^2 + (4 + 2 |m| )p + 4 + 4 |m|}
	\\
&=  2\frac{
	p - ( \varepsilon -  |m| - 1)  
}{p^2 + (4 + 2 |m| )p + 4 + 4 |m|}
&
c_{p+2}
&=  2\frac{
	p - ( \varepsilon -  |m| - 1)  
}{p^2 + (4 + 2 |m| )p + 4 + 4 |m|}
	\\
&\text{for $\varepsilon = 2n +|m| +1$}\implies  2\frac{
	p - ( 2n +|m| +1  -  |m| - 1)  
}{p^2 + (4 + 2 |m| )p + 4 + 4 |m|}
	\\
&= 2\frac{
	p - 2n
}{p^2 + (4 + 2 |m| )p + 4 + 4 |m|}
	\\
&\implies c_{2n + 2} = 0 \impliedby p = 2n
\end{align*}




\subsection*{(c)}

\[
E(n_x, n_y) = \hb \omega \left(n_x + \frac{1}{2} + n_y + \frac{1}{2}\right)
\] 
\[
\begin{array}{|c|c|c|c|c|c|c|c|c|c|c|c|}
\hline
n_y \setminus n_x & 0 & 1 & 2 & 3 & 4 & 5 & 6 & 7 & 8 & 9 & 10 \\ \hline
0 & 1\hbar\omega & 2\hbar\omega & 3\hbar\omega & 4\hbar\omega & 5\hbar\omega & 6\hbar\omega & 7\hbar\omega & 8\hbar\omega & 9\hbar\omega & 10\hbar\omega & 11\hbar\omega \\ \hline
1 & 2\hbar\omega & 3\hbar\omega & 4\hbar\omega & 5\hbar\omega & 6\hbar\omega & 7\hbar\omega & 8\hbar\omega & 9\hbar\omega & 10\hbar\omega & 11\hbar\omega & 12\hbar\omega \\ \hline
2 & 3\hbar\omega & 4\hbar\omega & 5\hbar\omega & 6\hbar\omega & 7\hbar\omega & 8\hbar\omega & 9\hbar\omega & 10\hbar\omega & 11\hbar\omega & 12\hbar\omega & 13\hbar\omega \\ \hline
3 & 4\hbar\omega & 5\hbar\omega & 6\hbar\omega & 7\hbar\omega & 8\hbar\omega & 9\hbar\omega & 10\hbar\omega & 11\hbar\omega & 12\hbar\omega & 13\hbar\omega & 14\hbar\omega \\ \hline
4 & 5\hbar\omega & 6\hbar\omega & 7\hbar\omega & 8\hbar\omega & 9\hbar\omega & 10\hbar\omega & 11\hbar\omega & 12\hbar\omega & 13\hbar\omega & 14\hbar\omega & 15\hbar\omega \\ \hline
5 & 6\hbar\omega & 7\hbar\omega & 8\hbar\omega & 9\hbar\omega & 10\hbar\omega & 11\hbar\omega & 12\hbar\omega & 13\hbar\omega & 14\hbar\omega & 15\hbar\omega & 16\hbar\omega \\ \hline
6 & 7\hbar\omega & 8\hbar\omega & 9\hbar\omega & 10\hbar\omega & 11\hbar\omega & 12\hbar\omega & 13\hbar\omega & 14\hbar\omega & 15\hbar\omega & 16\hbar\omega & 17\hbar\omega \\ \hline
7 & 8\hbar\omega & 9\hbar\omega & 10\hbar\omega & 11\hbar\omega & 12\hbar\omega & 13\hbar\omega & 14\hbar\omega & 15\hbar\omega & 16\hbar\omega & 17\hbar\omega & 18\hbar\omega \\ \hline
8 & 9\hbar\omega & 10\hbar\omega & 11\hbar\omega & 12\hbar\omega & 13\hbar\omega & 14\hbar\omega & 15\hbar\omega & 16\hbar\omega & 17\hbar\omega & 18\hbar\omega & 19\hbar\omega \\ \hline
9 & 10\hbar\omega & 11\hbar\omega & 12\hbar\omega & 13\hbar\omega & 14\hbar\omega & 15\hbar\omega & 16\hbar\omega & 17\hbar\omega & 18\hbar\omega & 19\hbar\omega & 20\hbar\omega \\ \hline
10 & 11\hbar\omega & 12\hbar\omega & 13\hbar\omega & 14\hbar\omega & 15\hbar\omega & 16\hbar\omega & 17\hbar\omega & 18\hbar\omega & 19\hbar\omega & 20\hbar\omega & 21\hbar\omega \\ \hline
\end{array}
\]
This is clear as day to notice that for $\Pi \hb \omega$ there are $\Pi$ entries. We can just count diagonally.  
\[
E(n,m) = \hb \omega \left(2 n + |m| + 1\right)
\] 
\[
\begin{array}{|c|c|c|c|c|c|c|c|c|c|c|c|}
\hline
n \setminus |m| & 0 & 1 & 2 & 3 & 4 & 5 & 6 & 7 & 8 & 9 & 10 \\ \hline
0 & 1\hbar\omega & 2\hbar\omega & 3\hbar\omega & 4\hbar\omega & 5\hbar\omega & 6\hbar\omega & 7\hbar\omega & 8\hbar\omega & 9\hbar\omega & 10\hbar\omega & 11\hbar\omega \\ \hline
1 & 3\hbar\omega & 4\hbar\omega & 5\hbar\omega & 6\hbar\omega & 7\hbar\omega & 8\hbar\omega & 9\hbar\omega & 10\hbar\omega & 11\hbar\omega & 12\hbar\omega & 13\hbar\omega \\ \hline
2 & 5\hbar\omega & 6\hbar\omega & 7\hbar\omega & 8\hbar\omega & 9\hbar\omega & 10\hbar\omega & 11\hbar\omega & 12\hbar\omega & 13\hbar\omega & 14\hbar\omega & 15\hbar\omega \\ \hline
3 & 7\hbar\omega & 8\hbar\omega & 9\hbar\omega & 10\hbar\omega & 11\hbar\omega & 12\hbar\omega & 13\hbar\omega & 14\hbar\omega & 15\hbar\omega & 16\hbar\omega & 17\hbar\omega \\ \hline
4 & 9\hbar\omega & 10\hbar\omega & 11\hbar\omega & 12\hbar\omega & 13\hbar\omega & 14\hbar\omega & 15\hbar\omega & 16\hbar\omega & 17\hbar\omega & 18\hbar\omega & 19\hbar\omega \\ \hline
5 & 11\hbar\omega & 12\hbar\omega & 13\hbar\omega & 14\hbar\omega & 15\hbar\omega & 16\hbar\omega & 17\hbar\omega & 18\hbar\omega & 19\hbar\omega & 20\hbar\omega & 21\hbar\omega \\ \hline
6 & 13\hbar\omega & 14\hbar\omega & 15\hbar\omega & 16\hbar\omega & 17\hbar\omega & 18\hbar\omega & 19\hbar\omega & 20\hbar\omega & 21\hbar\omega & 22\hbar\omega & 23\hbar\omega \\ \hline
7 & 15\hbar\omega & 16\hbar\omega & 17\hbar\omega & 18\hbar\omega & 19\hbar\omega & 20\hbar\omega & 21\hbar\omega & 22\hbar\omega & 23\hbar\omega & 24\hbar\omega & 25\hbar\omega \\ \hline
8 & 17\hbar\omega & 18\hbar\omega & 19\hbar\omega & 20\hbar\omega & 21\hbar\omega & 22\hbar\omega & 23\hbar\omega & 24\hbar\omega & 25\hbar\omega & 26\hbar\omega & 27\hbar\omega \\ \hline
9 & 19\hbar\omega & 20\hbar\omega & 21\hbar\omega & 22\hbar\omega & 23\hbar\omega & 24\hbar\omega & 25\hbar\omega & 26\hbar\omega & 27\hbar\omega & 28\hbar\omega & 29\hbar\omega \\ \hline
10 & 21\hbar\omega & 22\hbar\omega & 23\hbar\omega & 24\hbar\omega & 25\hbar\omega & 26\hbar\omega & 27\hbar\omega & 28\hbar\omega & 29\hbar\omega & 30\hbar\omega & 31\hbar\omega \\ \hline
\end{array}
\]
\textbf{For $\hb \omega$}: 
In this case there is one entry for $m = 0, n = 0.$

\textbf{For $2 \hb \omega$}: 
In this case there is one entry for $m = 1, n = 0$ but we have to careful because $m  = - 1, n= 0$ is also another separate case, hence keeping 2 entries. 

\textbf{For $3 \hb \omega$ :  }
For this we are dealing with $ m= 2, 0$ for respective  $n$, and there is another term for $m = -2$. Hence keeping $3$ entries. 

We can go on like this for ever and count that for $\Pi \hb \omega$ we have $\Pi$ number of entries.

\newpage
\section*{Problem 02}
\hrule
\subsection*{(a)} 
\begin{align*}
\hat{x} &= \frac{1}{b} \hat{X} 
	&\hat{p} &= \frac{b}{\hb} \hat{P} \\
\end{align*}
\begin{align*}
	\hat{a} \ket{n = 0} &= 0 \\ 
	\frac{1}{\sqrt{2} }\left(\hat{x} + i \hat{p}\right) \ket{n = 0}= 0 \\
	\frac{1}{\sqrt{2} }\left( \hat{x} + i \hat{p}\right)\hat{I} \ket{n = 0}= 0 \\
	\frac{1}{\sqrt{2} }\left( \hat{x} + i \hat{p}\right)\ket{p} \braket{p | n=0}= 0 \\
	\implies
	\frac{1}{\sqrt{2} }\bra{p'}\left( \hat{x} + i \hat{p}\right)\ket{p} \braket{p | n=0}= 0 \\
	\frac{1}{\sqrt{2} }
	\Big[
		\bra{p'}\hat{x} \ket{p} + i \bra{p'}\hat{p}\ket{p}
	\Big] 
	\braket{p | n=0}= 0 \\
	\frac{1}{\sqrt{2} }
	\Big[
		\bra{p'}\hat{x} \ket{p} \psi_0(p) + i \bra{p'}\hat{p}\ket{p}
	\psi_0(p)
	\Big] = 0 \\
		i \hb \frac{1}{b} \frac{\mathrm{d} }{\mathrm{d} p} \psi_0(p) + 
\frac{b}{\hb}
		i p 
	\psi_0(p)
	= 0 \\
	\implies
		 \frac{\hb}{b} \frac{\mathrm{d} }{\mathrm{d} p} \psi_0(p) +  \frac{b}{\hb}p 
	\psi_0(p)
	= 0 \\
		 \frac{\hb^2}{b^2} \frac{\mathrm{d} }{\mathrm{d} p} \psi_0(p) +  p 
	\psi_0(p)
	= 0 \\
\frac{\hb^2}{b^2} \frac{\mathrm{d} \psi_0(p) }{\psi_0(p)} = - p \, \mathrm{d} p \\
\frac{\hb^2}{b^2} \ln \left(\frac{\psi_0(p)}{\psi_0(0)}\right)= - \frac{p^2}{2} \\
 \ln \left(\frac{\psi_0(p)}{\psi_0(0)}\right)= - \frac{b^2}{2 \hb^2 } p^2 \\
 \ln \left(\frac{\psi_0(p)}{\psi_0(0)}\right)= - \frac{\hb}{2 m \omega \hb^2 } p^2 \\
 \ln \left(\frac{\psi_0(p)}{\psi_0(0)}\right)= - \frac{p^2}{2  \omega  m \hb }  \\
 \psi_0(p) = \psi_0(0) \, \mathrm e^{- p^2 / 2 m \omega \hb }
\end{align*}




\begin{align*}
	| \psi_0(p)| ^2 =
\psi_0^2(0) \int_{-\infty}^{\infty} \mathrm{d} p \, 
e^{-p^2 / m \omega \hb} = \psi_0^2(0)  \frac{\sqrt{2 \pi } }{\sqrt{2 / m \omega \hb} } 
= \psi_0^2(0) \sqrt{m \omega \pi \hb} \\ 
\implies 
|\psi_0(p)|^2 = \psi_0^2(0) \sqrt{m \omega \pi \hb} \\ 
\implies
\Psi_0(p) = \frac{e^{-p^2 / 2 m \omega \hb } }{(m \omega \pi \hb)^{1 / 4} }
\end{align*}




\subsection*{(b)}
\begin{align*}
\psi_0(x) = 
\braket{x | n = 0} = 
\int_{-\infty}^{\infty} \braket{x | p} \braket{p | n = 0} \, \mathrm{d} p  &= 
\int_{-\infty}^{\infty} \frac{1}{\sqrt{2 \pi \hb}}e^{i p x / \hb} 
\Psi_0(p)
\, \mathrm{d} p  \\ 
&=  \frac{1}{\sqrt{2 \pi \hb}}\int_{-\infty}^{\infty} e^{i p x / \hb} 
\frac{e^{-p^2 / 2 m \omega \hb } }{(m \omega \pi \hb)^{1 / 4} }
\, \mathrm{d} p  \\ 
&= \frac{1}{\sqrt{2 \pi \hb}}\frac{1}{(m \omega \pi \hb)^{1 / 4}} \int_{-\infty}^{\infty} e^{i p x / \hb
{-p^2 / 2 m \omega \hb }} 
\, \mathrm{d} p  \\ 
&= \frac{1}{\sqrt{2 \pi \hb}}\frac{1}{(m \omega \pi \hb)^{1 / 4}} 
\int_{-\infty}^{\infty} 
e^{\beta p 
{- \frac{\alpha}{2} p^2 }} 
\, \mathrm{d} p  
\impliedby 
\begin{cases}
	\alpha &= \frac{1}{m \omega \hb } \\
	\beta &= \frac{ix}{\hb} \\
\end{cases}
\\ 
&= \frac{1}{\sqrt{2 \pi \hb}}\frac{1}{(m \omega \pi \hb)^{1 / 4}} 
\left(
\sqrt{\frac{2\pi}{\alpha}}  e^{\beta^2 / 2 \alpha}
\right)
\impliedby 
\begin{cases}
	\alpha &= \frac{1}{m \omega \hb } \\
	\beta &= \frac{ix}{\hb} \\
\end{cases} \\ 
&= \frac{1}{\sqrt{2 \pi \hb}}\frac{1}{(m \omega \pi \hb)^{1 / 4}} 
\left(
	\sqrt{2 \pi m \omega \hb }  \, 
e^{- x ^2 (m \omega \hb )/ 2 \hb^2}
\right)\\ 
&= \frac{1}{\sqrt{2 \pi \hb}}\frac{1}{(m \omega \pi \hb)^{1 / 4}} 
\left(
	\sqrt{2 \pi m \omega \hb }  \, 
e^{- x ^2 (m \omega )/ 2 \hb}
\right) \\ 
&= \frac{1}{\sqrt{2 \pi \hb}}\frac{1}{(m \omega \pi \hb)^{1 / 4}} 
\left(
	\sqrt{2 \pi m \omega \hb }  \, 
e^{- x ^2/ 2 b}
\right) \\ 
&= \frac{\sqrt{m \omega } }{(m \omega \pi \hb)^{1 / 4}} 
\left(\, 
e^{- x ^2/ 2 b}
\right) \\ 
&= \frac{({m \omega } )^{1 / 4}}{(\pi \hb)^{1 / 4}} 
\left(\, 
e^{- x ^2/ 2 b}
\right) \\ 
&= 
\frac{1}{\pi^{1 / 4} b^{ 1 / 2}}
e^{- x ^2/ 2 b}
\end{align*}
























\newpage
\section*{Problem 03} 
\hrule
\subsection*{(a)} 
\textbf{For $n=1$ :}
\begin{align*}
	\left(y - \frac{\mathrm{d} }{\mathrm{d} y}\right) e^{-y^2 / 2}
	&= y e^{-y^2 / 2} - \frac{\mathrm{d} }{\mathrm{d} y} e^{-y ^2 / 2}  \\
	&= 
	ye^{- y^2 / 2}  + 
	ye^{- y^2 / 2} 
	\\
	&= 
	2 ye^{- y^2 / 2} 
\end{align*}




\textbf{For $n=2$ :}
\begin{align*}
	\left(y - \frac{\mathrm{d} }{\mathrm{d} y}\right)^2 e^{- y^2 / 2}
	&=  
	\left(y - \frac{\mathrm{d} }{\mathrm{d} y}\right)
	\left(y - \frac{\mathrm{d} }{\mathrm{d} y}\right) e^{- y^2 / 2} \\ 
	&=
	\left(y - \frac{\mathrm{d} }{\mathrm{d} y}\right) 
	2 y e^{ - y^2 / 2} \\ 
	&= 
2y^2 e^{- y^2 / 2} - 
\frac{\mathrm{d} }{\mathrm{d} y} 
\left(
2 y e^{- y^2 / 2}
\right)
	\\
	&= 
2 y^2 e^{- y^2 / 2} 
- 
\left(
2 e ^{ - y ^2 / 2} 
- 
2 y^2 e^{- y^2 / 2}
\right)
	\\ 
	&= 
4 y^2 e^{- y ^2 / 2} - 2 e^{ - y ^2 / 2} 
	\\
	&= (4 y^2 - 2)e^{- y^2 / 2} \\
\end{align*}


\begin{align*}
	\psi_1(x) 
	&= 
	\frac{2 y e ^{ - y ^2 / 2}}{\sqrt{2 b\sqrt{\pi} }  } \tag{$y = x / b$}
	\\
	\psi_2(x) 
	&= 
\frac{(4 y^2 - 2) e^{ - y ^2 / 2}}{2 \sqrt{2b\sqrt{\pi} } }
	\\
\end{align*}



\subsection*{(b)} 

\begin{align*}
\int_{-\infty}^{\infty} 
\mathrm{d} x \, 
e^{-  \alpha x^2 / 2} 
&= 
\sqrt{\frac{2\pi}{a}} \\
\frac{\mathrm{d} }{\mathrm{d} \alpha }\int_{-\infty}^{\infty} 
\mathrm{d} x \, 
e^{-  \alpha x^2 / 2} 
&= 
\frac{\mathrm{d} }{\mathrm{d} \alpha}
\sqrt{\frac{2\pi}{a}} \\
\int_{-\infty}^{\infty} 
\mathrm{d} x \, 
\frac{\mathrm{d} }{\mathrm{d} \alpha }
e^{-  \alpha x^2 / 2}  
&= 
\sqrt{2 \pi }  \left(
- \frac{1}{2} a^{- \frac{3}{2}}
\right) \\
- \frac{1}{2 } 
\int_{-\infty}^{\infty} 
\mathrm{d} x \, 
x^2 e^{-  \alpha x^2 / 2}  
&= 
\frac{\sqrt{2 \pi } }{a^{\frac{3}{2}}}  \left(
- \frac{1}{2} 
\right)\\
\int_{-\infty}^{\infty} 
\mathrm{d} x \, 
x^2 e^{-  \alpha x^2 / 2}  
&= 
\frac{\sqrt{2 \pi } }{a^{{3}/ {2}}} 
\end{align*}





\subsection*{(c)} 
Consider the functions without the normalization constants in front
\begin{align*}
	\Psi_0(x) &= e^{ - y^2 / 2} \\ 
	\Psi_1(x) &= y e^{ - y^2 / 2} \\
	\Psi_2(x) &= (4 y^2 - 2) e^{ - y^2  / 2} \\
\end{align*}
\begin{align*}
\braket{0 | 2 }
&\implies
\int_{-\infty}^{\infty} \mathrm{d} y \, 
(4 y^2 - 2) e^{ - y^2 } \\
&= \int_{-\infty}^{\infty} \mathrm{d} y \, 
4 y^2 e^{ - y^2 } - 
\int_{-\infty}^{\infty} \mathrm{d} y \, 2 e^{ - y^2 }\\
&= 
\sqrt{2\pi } 
\left(
\frac{4}{2^{3 / 2}} 
- 
\frac{2}{2^{1 / 2}}
\right)
\\
&= 
\sqrt{2\pi } 
\left(
\frac{2}{2^{1 / 2}} 
- 
\frac{2}{2^{1 / 2}}
\right) = 0
\end{align*}




\begin{align*}
\braket{1 | 1} 
&= 
\int_{-\infty}^{\infty} 
\mathrm{d} x \, 
y^2 e^{ - y^2 } 
\\
&= b
\int_{-\infty}^{\infty} 
\mathrm{d} y \, 
y^2 e^{ - y^2 }  \\ 
&=b \frac{\sqrt{2 \pi } }{2^{3 / 2}} \\
&= b \frac{\sqrt{2} \sqrt{\pi} }{\sqrt{2} ^{3}} = b \frac{ \sqrt{\pi}  }{2} \\
\end{align*}
Coefficients of $\Psi_1(x)$ are 
\[
C = \frac{2}{ \sqrt{2b \sqrt{\pi} } } \implies C^2
= 
\frac{2}{b \sqrt{\pi} }
\] 
Putting that in place 
\[
\braket{1 | 1} = C^2 \int_{-\infty}^{\infty} \mathrm{d} x \, y^2 e^{- y^2}  = \frac{2}{b \sqrt{\pi } } b \frac{\sqrt{\pi } }{2} = 1
\] 



























\newpage
\section*{Problem 04} 
\hrule 
\subsection*{(a)} 
\begin{align*}
	\hat{\overline{X}} &= \frac{1}{\sqrt{2} } (\hat{a} + \hat{a}^{T}) 
			   &
			   \hat{\overline{P}} &= \frac{i}{\sqrt{2} } (\hat{a}^{T} - \hat{a}) \\
\hat{\overline{X}} \hat{\overline{X}} 
					      &= \frac{1}{2} 
					      \left(\hat{a} + \hat{a}^{T}\right)
					      \left(\hat{a}+ \hat{a}^{T}\right) 
					      &
					    \hat{\overline{P}}
					    \hat{\overline{P}}
					    &= -
					    \frac{1}{2} 
					    \left(\hat{a}^{T} - \hat{a}\right)
					    \left(\hat{a}^{T} - \hat{a}\right) 
					 \\ &=
					    \frac{1}{2}
					    \left(
					    \hat{a}\hat{a}
				    + \hat{a}^{T}\hat{a}^{T}
			    + \hat{a}^{T} \hat{a} + 
		    \hat{a} \hat{a}^{T}\right)
					    & &=-\frac{1}{2} 
					    \left(
					    \hat{a}\hat{a}
				    + \hat{a}^{T}\hat{a}^{T}
			    - \hat{a}^{T} \hat{a} - 
		    \hat{a} \hat{a}^{T} 
					    \right)
\end{align*}



\begin{align*}
\bra{n} \hat{\overline{X}} \ket{n} &= 
\frac{1}{\sqrt{2} }
\bra{n} \hat{a} + \hat{a}^{T} \ket{n}
\\
&= \frac{1}{\sqrt{2} }
\left(
\braket{n | \hat{a} | n} + 
\braket{n | \hat{a}^{T} | n }
\right) \\
&= 
\frac{1}{\sqrt{2} }
\left(
\sqrt{n} \braket{n | n-1} +
\sqrt{n+1} \braket{n | n+1}
\right) = 0
\\
\braket{n | \hat{\overline{P}} | n} &= 
\frac{i}{\sqrt{2} } 
\braket{n | \hat{a}^{T} - \hat{a} | n}
\\
				    &=
\frac{i}{\sqrt{2} } 
\left(
\braket{n | \hat{a}^{T} | n} - 
\braket{n | \hat{a} | n}
\right) = 0
\end{align*}


\begin{align*}
\bra{n} \hat{\overline{X}}^2  \ket{ n} 
&= 
\frac{1}{2}
\left(
\braket{ n | \hat{a} \hat{a} | n}
+
\braket{n | \hat{a}^{T} \hat{a}^{T} | n} 
+ 
\braket{n | \hat{a} \hat{a}^{T} | n	}
+
\braket{n | \hat{a}^{T} \hat{a} | n} 
\right)\\
&= 
\frac{1}{2}
\left(
0 + 0 + (n+1) + n 
\right)
\\
&= 
\frac{1}{2} 
\left(2n + 1\right)
\\
&= n + \frac{1}{2}  \\
\
\
\
\bra{n} \hat{\overline{P}} ^2 \ket{ n} 
&= -
\frac{1}{2}
\left(
\braket{ n | \hat{a} \hat{a} | n}
+
\braket{n | \hat{a}^{T} \hat{a}^{T} | n} 
- 
\braket{n | \hat{a} \hat{a}^{T} | n	}
-
\braket{n | \hat{a}^{T} \hat{a} | n} 
\right)\\
&= - \frac{1}{2} 
\left(
0 + 0 - \left(
	(n+1) + n
\right)
\right)\\
& = n + \frac{1}{2}
\end{align*}



\begin{align*}
\Delta X  
&= \sqrt{\frac{\hb}{m \omega}} 
\sqrt{
\braket{n | \hat{\overline{X}}^2 | n }
-
\braket{n | \hat{\overline{X} } | n}
} = \sqrt{\frac{\hb}{m \omega } } 
\sqrt{n + \frac{1}{2}} \\
\Delta P  
&= \hb \sqrt{\frac{m \omega }{\hb}}  
\sqrt{
\braket{n | \hat{\overline{P}}^2 | n }
-
\braket{n | \hat{\overline{P} } | n}
} = \hb \sqrt{\frac{m \omega }{ \hb } } 
\sqrt{n + \frac{1}{2}} \\
\end{align*}


\subsection*{(b)}
\begin{align*} \implies
	\Delta X \Delta P &= \hb \left(n + \frac{1}{2}\right) \\ 
	\Delta X \Delta P &\ge \frac{\hb}{2} \\ 
	\Delta X \Delta P &= \frac{\hb}{2} \iff  n = 0
\end{align*}










\newpage
\section*{Problem 05} 
\hrule
\begin{align*}
	\frac{\mathrm{d} }{\mathrm{d} t} 
	\braket{ \Omega} (t) &= 
	\frac{i}{\hb} 
	\braket{ [H, \Omega] } (t)\\
	\frac{\mathrm{d} }{\mathrm{d} t} 
	\braket{ a} (t) &= 
	\frac{i}{\hb} 
	\braket{ [H, a] } (t)\\
	&= 
	\frac{i}{\hb} 
	\braket{ \left[ \hb \omega \left(a^{T} a + \frac{1}{2} I \right), a \right]}\\
	&= 
	i \omega 
	\braket{ \left[ \left(a^{T} a \right), a \right]}\\
	&= 
	- i \omega 
	\braket{ a } \\
	\int \frac{1}{\braket{ a}}\frac{\mathrm{d} }{\mathrm{d} t} \braket{ a } \, \mathrm{d} t &= 
	\int
	- i \omega 
	  \, \mathrm{d}  t\\
	\braket{ a} (t) &= \braket{ a}(0) e^{- i \omega t}
\end{align*}

\subsection*{Scratchwork}
\hrule
\begin{align*}
	\frac{\mathrm{d} }{\mathrm{d} t} 
	\braket{ \Omega} (t) &= 
	\frac{i}{\hb} 
	\braket{ [H, \Omega] } (t)\\
	\frac{\mathrm{d} }{\mathrm{d} t} 
	\braket{ a} (t) &= 
	\frac{i}{\hb} 
	\braket{ [H, a] } (t)\\
	&= 
	\frac{i}{\hb} 
	\bra{\psi} Ha - a H \ket{\psi}\\
	&= 
	\frac{i}{\hb} \left[
	\bra{\psi} Ha \ket{\psi}  - \bra{\psi} a H \ket{\psi}\right] \\
	&= 
	\frac{i (\hb \omega )}{\hb} \left[
\bra{\psi} \left(a^{T} a + \frac{1}{2} I \right)a \ket{\psi}  - \bra{\psi} a  \left(a^{T} a + \frac{1}{2} I \right)\ket{\psi}\right] \\
	&= 
	 i \omega \left[
\bra{\psi} a^{T} a a  \ket{\psi}  - \bra{\psi} a  a^{T} a \ket{\psi}\right] \\
	&= 
	 i \omega \left[
	 \bra{\psi(n)} a^{T} a a  \ket{\psi(n)}  - \bra{\psi(n)} a  a^{T} a \ket{\psi(n)}\right] \tag{rewrite with $n$-th energy eigenstate} \\
	&= 
	 i \omega \left[ \sqrt{n-1} 
	 \bra{\psi(n)} a^{T} a  \ket{\psi(n-1)}  - \sqrt{n-1} \bra{\psi(n)} a  a^{T}  \ket{\psi(n-1)}\right]\\ 
	&= 
	 i \omega \left[ \sqrt{(n-2)(n-1)} 
	 \bra{\psi(n)} a^{T}   \ket{\psi(n-2)}  - \sqrt{n (n-1)} \bra{\psi(n)} a \ket{\psi(n)}\right]\\ 
	&= 
	 i \omega \left[ \sqrt{(n-2)(n-1)^2} 
	 \bra{\psi(n)}   \ket{\psi(n-1)}  - \sqrt{n (n-1)^2} \bra{\psi(n)}  \ket{\psi(n-1)}\right]\\
	&= 
	 i \omega \left[ \sqrt{(n-2)(n-1)^2} 
	  - \sqrt{n (n-1)^2} \right] \braket{\psi(n) | \psi(n-1)}
\end{align*}




\end{document}
